F_mu_ref_conc/examples/lock.v
@@ -1,10 +1,10 @@
 From iris.proofmode Require Import invariants ghost_ownership tactics.
 From iris_logrel.F_mu_ref_conc Require Export rules_binary typing.
 
-Definition newlock : expr := Alloc (♭ false).
+Definition newlock : expr := Alloc (#♭ false).
 Definition acquire : expr :=
-  Rec (If (CAS (Var 1) (♭ false) (♭ true)) (Unit) (App (Var 0) (Var 1))).
-Definition release : expr := Rec (Store (Var 1) (♭ false)).
+  Rec (If (CAS (Var 1) (#♭ false) (#♭ true)) (Unit) (App (Var 0) (Var 1))).
+Definition release : expr := Rec (Store (Var 1) (#♭ false)).
 
 Definition with_lock (e : expr) (l : expr) : expr :=
   Rec
@@ -79,7 +79,7 @@ Section proof.
   Lemma steps_newlock E ρ j K :
     nclose specN ⊆ E →
     spec_ctx ρ ★ j ⤇ fill K newlock
-      ={E}=> ∃ l, j ⤇ fill K (Loc l) ★ l ↦ₛ (♭v false).
+      ={E}=> ∃ l, j ⤇ fill K (Loc l) ★ l ↦ₛ (#♭v false).
   Proof.
     iIntros {HNE} "[#Hspec Hj]".
     by iPvs (step_alloc _ _ j K with "[Hj]") as "Hj"; eauto.
@@ -89,8 +89,8 @@ Section proof.
 
   Lemma steps_acquire E ρ j K l :
     nclose specN ⊆ E →
-    spec_ctx ρ ★ l ↦ₛ (♭v false) ★ j ⤇ fill K (App acquire (Loc l))
-      ={E}=> j ⤇ fill K Unit ★ l ↦ₛ (♭v true).
+    spec_ctx ρ ★ l ↦ₛ (#♭v false) ★ j ⤇ fill K (App acquire (Loc l))
+      ={E}=> j ⤇ fill K Unit ★ l ↦ₛ (#♭v true).
   Proof.
     iIntros {HNE} "[#Hspec [Hl Hj]]". unfold acquire.
     iPvs (step_rec _ _ j K with "[Hj]") as "Hj"; eauto. done.
@@ -110,8 +110,8 @@ Section proof.
 
   Lemma steps_release E ρ j K l b:
     nclose specN ⊆ E →
-    spec_ctx ρ ★ l ↦ₛ (♭v b) ★ j ⤇ fill K (App release (Loc l))
-      ={E}=> j ⤇ fill K Unit ★ l ↦ₛ (♭v false).
+    spec_ctx ρ ★ l ↦ₛ (#♭v b) ★ j ⤇ fill K (App release (Loc l))
+      ={E}=> j ⤇ fill K Unit ★ l ↦ₛ (#♭v false).
   Proof.
     iIntros {HNE} "[#Hspec [Hl Hj]]". unfold release.
     iPvs (step_rec _ _ j K with "[Hj]") as "Hj"; eauto; try done.
@@ -126,11 +126,11 @@ Section proof.
   Lemma steps_with_lock E ρ j K e l P Q v w:
     nclose specN ⊆ E →
     (∀ f, e.[f] = e) (* e is a closed term *) →
-    (∀ K', spec_ctx ρ ★ P ★ j ⤇ fill K' (App e (# w))
-            ={E}=> j ⤇ fill K' (# v) ★ Q) →
-    spec_ctx ρ ★ P ★ l ↦ₛ (♭v false)
-                ★ j ⤇ fill K (App (with_lock e (Loc l)) (# w))
-      ={E}=> j ⤇ fill K (# v) ★ Q ★ l ↦ₛ (♭v false).
+    (∀ K', spec_ctx ρ ★ P ★ j ⤇ fill K' (App e (of_val w))
+            ={E}=> j ⤇ fill K' (of_val v) ★ Q) →
+    spec_ctx ρ ★ P ★ l ↦ₛ (#♭v false)
+                ★ j ⤇ fill K (App (with_lock e (Loc l)) (of_val w))
+      ={E}=> j ⤇ fill K (of_val v) ★ Q ★ l ↦ₛ (#♭v false).
   Proof.
     iIntros {HNE H1 H2} "[#Hspec [HP [Hl Hj]]]".
     iPvs (step_rec _ _ j K _ _ _ _ with "[Hj]") as "Hj"; eauto.
